feature: introduce the notion of value
Before this patch, the notion of memory location value was completely
absent. We introduce this notion within the Event type as a first
step towards true values handling.

src/Cache/Cache_def.v
@@ -1,5 +1,4 @@
-Require Import Coq.Structures.DecidableType.
-
+Require Import SpecCert.Equality.
 Require Import SpecCert.Address.
 Require Import SpecCert.Map.
 
@@ -14,25 +13,21 @@ Parameter eq_index_eq: forall i i':Index, i = i' -> index_eq i i'.
 
 Parameter phys_to_index: PhysicalAddress -> Index.
 
-Module IndexDec <: DecidableType with Definition t:= Index.
-  Definition t := Index.
+Instance IndexEq: Eq Index :=
+  { eq := index_eq
+  ; eq_sym := index_eq_sym
+  ; eq_refl := index_eq_refl
+  ; eq_trans := index_eq_trans
+  ; eq_dec := index_dec }.
 
-  Definition eq := index_eq.
-  Definition eq_refl := index_eq_refl.
-  Definition eq_sym := index_eq_sym.
-  Definition eq_trans := index_eq_trans.
-  Definition eq_dec := index_dec.
-End IndexDec.
-
-Record CacheEntry (S :Set) := {
-                      dirty: bool;
-                      content: S;
-                      tag: PhysicalAddress
-                    }.
+Record CacheEntry
+       (S: Type)
+  := { dirty: bool
+     ; content: S
+     ; tag: PhysicalAddress }.
 
 Arguments dirty   : default implicits.
 Arguments content : default implicits.
 Arguments tag     : default implicits.
 
-Module _IndexMap := Map (IndexDec).
-Definition Cache (S:Set) := _IndexMap.Map (CacheEntry S).
+Definition Cache (S: Type) := Map Index (CacheEntry S).
