src/Cache/Cache_func.v
@@ -1,9 +1,10 @@
 Require Import SpecCert.Cache.Cache_def.
 Require Import SpecCert.Cache.Cache_prop.
 Require Import SpecCert.Address.
+Require Import SpecCert.Map.
 
 Definition load_in_cache
-           {S     :Set}
+           {S     :Type}
            (cache :Cache S)
            (pa    :PhysicalAddress)
            (owner :S)
@@ -12,10 +13,10 @@ Definition load_in_cache
   let o' := {| dirty   := false
              ; content := owner
              ; tag     := pa |} in
-  _IndexMap.add_in_map cache (phys_to_index pa) o'.
+  add_in_map cache (phys_to_index pa) o'.
 
 Definition update_in_cache
-           {S     :Set}
+           {S     :Type}
            (cache :Cache S)
            (pa    :PhysicalAddress)
            (owner :S)
@@ -24,10 +25,10 @@ Definition update_in_cache
   let o' := {| dirty := true
              ; content := owner
              ; tag := pa |} in
-  _IndexMap.add_in_map cache (phys_to_index pa) o'.
+  add_in_map cache (phys_to_index pa) o'.
 
 Program Definition global_update_in_cache
-           {S     :Set}
+           {S     :Type}
            (cache :Cache S)
            (pa    :PhysicalAddress)
            (owner :S)
@@ -38,25 +39,25 @@ Program Definition global_update_in_cache
     load_in_cache cache pa owner _.
 
 Definition find_in_cache
-           {S     :Set}
+           {S     :Type}
            (cache :Cache S)
            (pa    :PhysicalAddress)
            :option S :=
   if cache_hit_dec cache pa then
-    Some (content (_IndexMap.find_in_map cache (phys_to_index pa)))
+    Some (content (find_in_map cache (phys_to_index pa)))
   else
     None.
 
 Definition find_in_cache_location
-           {S     :Set}
+           {S     :Type}
            (cache :Cache S)
            (pa    :PhysicalAddress)
            :S :=
-  content (_IndexMap.find_in_map cache (phys_to_index pa)).
+  content (find_in_map cache (phys_to_index pa)).
 
 Definition cache_location_address
-           {S     :Set}
+           {S     :Type}
            (cache :Cache S)
            (pa    :PhysicalAddress)
            :PhysicalAddress :=
-  tag (_IndexMap.find_in_map cache (phys_to_index pa)).
+  tag (find_in_map cache (phys_to_index pa)).
