src/Smm/Delta/Preserve/Read.v
@@ -11,13 +11,13 @@ Require Import SpecCert.Smm.Software.
 Require Import SpecCert.x86.
 
 Lemma read_strat_uc:
-  forall pa :PhysicalAddress,
-      partial_preserve (software (Read pa))
+  forall (pa :PhysicalAddress) (v: Value),
+      partial_preserve (software (Read pa v))
                        (fun a => resolve_cache_strategy (proc a) pa = Uncachable)
                        inv.
 Proof.
   unfold partial_preserve.
-  intros pa a a' Hinv Hres Hpre Hpost.
+  intros pa v a a' Hinv Hres Hpre Hpost.
   unfold x86_postcondition, read_post in Hpost.
   rewrite Hres in Hpost.
   unfold read_uncachable_post in Hpost.
@@ -26,13 +26,13 @@ Proof.
 Qed.
 
 Lemma read_strat_sh:
-  forall pa :PhysicalAddress,
-      partial_preserve (software (Read pa))
+  forall (pa :PhysicalAddress) (v: Value),
+      partial_preserve (software (Read pa v))
                        (fun a => resolve_cache_strategy (proc a) pa = SmrrHit)
                        inv.
 Proof.
   unfold partial_preserve.
-  intros pa a a' Hinv Hres Hpre Hpost.
+  intros pa v a a' Hinv Hres Hpre Hpost.
   unfold x86_postcondition, read_post in Hpost.
   rewrite Hres in Hpost.
   unfold read_smrrhit_post in Hpost.
@@ -41,14 +41,14 @@ Proof.
 Qed.
 
 Lemma read_strat_smrr_wb:
-  forall pa :PhysicalAddress,
-      partial_preserve (software (Read pa))
+  forall (pa :PhysicalAddress) (v: Value),
+      partial_preserve (software (Read pa v))
                        (fun a => is_inside_smrr (proc a) pa
                               /\ smm_strategy (smrr (proc a)) = WriteBack)
                        inv.
 Proof.
   unfold partial_preserve.
-  intros pa a a' Hinv [Hsmrr Hsmm] Hpre Hpost.
+  intros pa v a a' Hinv [Hsmrr Hsmm] Hpre Hpost.
   unfold x86_postcondition, read_post, resolve_cache_strategy in Hpost.
   destruct is_inside_smrr_dec; [| intuition ].
   destruct is_in_smm_dec.
@@ -66,13 +66,13 @@ Proof.
 Qed.
 
 Lemma read_strat_not_smrr:
-  forall pa :PhysicalAddress,
-      partial_preserve (software (Read pa))
+  forall (pa :PhysicalAddress) (v: Value),
+      partial_preserve (software (Read pa v))
                        (fun a => ~ is_inside_smrr (proc a) pa)
                        inv.
 Proof.
   unfold partial_preserve.
-  intros pa a a' Hinv Hnot_smrr Hpre Hpost.
+  intros pa v a a' Hinv Hnot_smrr Hpre Hpost.
   unfold x86_postcondition, read_post in Hpost.
   unfold resolve_cache_strategy in Hpost.
   destruct is_inside_smrr_dec; [ intuition |].
@@ -95,13 +95,13 @@ Proof.
 Qed.
 
 Lemma read_inv:
-  forall pa :PhysicalAddress,
-      preserve (software (Read pa)) inv.
+  forall (pa :PhysicalAddress) (v: Value),
+      preserve (software (Read pa v)) inv.
 Proof.
   unfold preserve.
-  intros pa a a' Hinv Hpre Hpost.
+  intros pa v a a' Hinv Hpre Hpost.
   case_eq (resolve_cache_strategy (proc a) pa); intro Heqstrat.
-  + apply (read_strat_uc pa a a' Hinv Heqstrat Hpre Hpost).
+  + apply (read_strat_uc pa v a a' Hinv Heqstrat Hpre Hpost).
   + destruct (is_inside_smrr_dec (proc a) pa).
     * unfold resolve_cache_strategy in Heqstrat.
       destruct is_inside_smrr_dec; [| intuition ].
@@ -109,18 +109,18 @@ Proof.
       assert (is_inside_smrr (proc a) pa /\ smm_strategy (smrr (proc a)) = WriteBack); [
           split; trivial
          |].
-      apply (read_strat_smrr_wb pa a a' Hinv H Hpre Hpost).
-    * apply (read_strat_not_smrr pa a a' Hinv n Hpre Hpost).
-  + apply (read_strat_sh pa a a' Hinv Heqstrat Hpre Hpost).
+      apply (read_strat_smrr_wb pa v a a' Hinv H Hpre Hpost).
+    * apply (read_strat_not_smrr pa v a a' Hinv n Hpre Hpost).
+  + apply (read_strat_sh pa v a a' Hinv Heqstrat Hpre Hpost).
 Qed.
 
 Lemma exec_inv:
-  forall o :Software,
-    preserve (hardware (Exec o)) inv.
+  forall (v: Value),
+    preserve (hardware (Exec v)) inv.
 Proof.
   unfold preserve.
-  intros o a a' Hinv Hpre Hpost.
-  apply (read_inv (ip (proc a)) a a'); [ exact Hinv | idtac |].
+  intros v a a' Hinv Hpre Hpost.
+  apply (read_inv (ip (proc a)) v a a'); [ exact Hinv | idtac |].
   + unfold x86_precondition, no_pre; trivial.
   + unfold x86_postcondition in *; exact Hpost.
 Qed.
