src/Smm/Delta/Preserve/Write.v
@@ -12,13 +12,13 @@ Require Import SpecCert.Smm.Software.
 Require Import SpecCert.x86.
 
 Lemma write_strat_uc:
-  forall pa :PhysicalAddress,
-    partial_preserve (software (Write pa))
+  forall (pa :PhysicalAddress) (v: Value),
+    partial_preserve (software (Write pa v))
                      (fun a => resolve_cache_strategy (proc a) pa = Uncachable)
                      inv.
 Proof.
   unfold partial_preserve.
-  intros pa a a' Hinv Hsmm_strat Hpre Hpost.
+  intros pa v a a' Hinv Hsmm_strat Hpre Hpost.
   unfold x86_postcondition, write_post in Hpost.
   rewrite Hsmm_strat in Hpost.
   unfold write_uncachable in Hpost.
@@ -26,13 +26,13 @@ Proof.
 Qed.
 
 Lemma write_strat_sh:
-  forall pa :PhysicalAddress,
-    partial_preserve (software (Write pa))
+  forall (pa :PhysicalAddress) (v: Value),
+    partial_preserve (software (Write pa v))
                      (fun a => resolve_cache_strategy (proc a) pa = SmrrHit)
                      inv.
 Proof.
   unfold partial_preserve.
-  intros pa a a' Hinv Hsmm_strat Hpre Hpost.
+  intros pa v a a' Hinv Hsmm_strat Hpre Hpost.
   unfold x86_postcondition, write_post in Hpost.
   rewrite Hsmm_strat in Hpost.
   unfold write_smrrhit in Hpost.
@@ -41,14 +41,14 @@ Proof.
 Qed.
 
 Lemma write_strat_smrr_wb:
-  forall pa :PhysicalAddress,
-    partial_preserve (software (Write pa))
+  forall (pa :PhysicalAddress) (v: Value),
+    partial_preserve (software (Write pa v))
                      (fun a => is_inside_smrr (proc a) pa
                             /\ smm_strategy (smrr (proc a)) = WriteBack)
                      inv.
 Proof.
   unfold partial_preserve.
-  intros pa a a' Hinv [Hinside_smrr Hsmm_strat] Hpre Hpost.
+  intros pa v a a' Hinv [Hinside_smrr Hsmm_strat] Hpre Hpost.
   unfold x86_postcondition, write_post, resolve_cache_strategy in Hpost.
   destruct is_inside_smrr_dec; [| intuition ].
   destruct is_in_smm_dec as [Hin_smm|Hnot].
@@ -80,13 +80,13 @@ Proof.
 Qed.
 
 Lemma write_not_smrr:
-  forall pa :PhysicalAddress,
-    partial_preserve (software (Write pa))
+  forall (pa :PhysicalAddress) (v: Value),
+    partial_preserve (software (Write pa v))
                      (fun a => ~ is_inside_smrr (proc a) pa)
                      inv.
 Proof.
   unfold partial_preserve.
-  intros pa a a' Hinv Hnot_inside_smrr Hpre Hpost.
+  intros pa v a a' Hinv Hnot_inside_smrr Hpre Hpost.
   unfold x86_postcondition in Hpost;
   unfold x86_precondition in Hpre.
   assert (write_post smm_context pa a a') as Hx; [unfold x86_postcondition in Hpost; exact Hpost |].
@@ -97,7 +97,7 @@ Proof.
   destruct is_inside_smrr_dec; [ intuition |].
   exact Heqstrat.
   case_eq (resolve_cache_strategy (proc a) pa); intro Hres; rewrite Hres in Hpost.
-  + apply (write_strat_uc pa a a' Hinv Hres Hpre Hx).
+  + apply (write_strat_uc pa v a a' Hinv Hres Hpre Hx).
   + destruct (is_inside_smrr_dec (proc a) pa); [ intuition |].
     unfold write_writeback in Hpost.
     assert (is_inside_smram pa -> is_in_smm (proc a)).
@@ -109,25 +109,25 @@ Proof.
     destruct (cache_hit_dec (cache a) pa).
     * apply (update_cache_content_with_context_preserves_inv a a' pa Hinv H0 Hpost).
     * apply (load_then_update_cache_with_context_preserves_inv a a' pa Hinv H0 Hpost).
- + apply (write_strat_sh pa a a' Hinv Hres Hpre Hx).
+ + apply (write_strat_sh pa v a a' Hinv Hres Hpre Hx).
 Qed.
 
 Lemma write_inv:
-  forall pa :PhysicalAddress,
-    preserve (software (Write pa)) inv.
+  forall (pa :PhysicalAddress) (v: Value),
+    preserve (software (Write pa v)) inv.
 Proof.
   unfold preserve.
-  intros pa a a' Hinv Htrans.
+  intros pa v a a' Hinv Htrans.
   destruct (is_inside_smrr_dec (proc a) pa).
   + case_eq (resolve_cache_strategy (proc a) pa); intro Hres.
-    * apply (write_strat_uc pa a a' Hinv Hres Htrans).
+    * apply (write_strat_uc pa v a a' Hinv Hres Htrans).
     * assert (is_inside_smrr (proc a) pa /\ smm_strategy (smrr (proc a)) = WriteBack).
       split; [ exact i |].
       unfold resolve_cache_strategy in Hres.
       destruct is_inside_smrr_dec; [| intuition ].
       destruct is_in_smm_dec; [| discriminate Hres ].
       exact Hres.
-      apply (write_strat_smrr_wb pa a a' Hinv H Htrans).
-    * apply (write_strat_sh pa a a' Hinv Hres Htrans).
-  + apply (write_not_smrr pa a a' Hinv n Htrans).
+      apply (write_strat_smrr_wb pa v a a' Hinv H Htrans).
+    * apply (write_strat_sh pa v a a' Hinv Hres Htrans).
+  + apply (write_not_smrr pa v a a' Hinv n Htrans).
 Qed.
