src/x86/Transition/Transition_def.v
@@ -27,37 +27,37 @@ Definition id_post
 Definition x86_precondition
            {S:  Set}
            (h:  Architecture S)
-           (ev: x86Event S)
+           (ev: x86Event)
   : Prop :=
   match ev with
   | software DisableInterrupt     => no_pre
   | software EnableInterrupt      => no_pre
-  | software (Write addr)         => no_pre
-  | software (Read addr)          => no_pre
+  | software (Write addr value)   => no_pre
+  | software (Read addr value)    => no_pre
   | software OpenSmram            => open_smram_pre
   | software CloseSmram           => close_smram_pre
   | software LockSmramc           => lock_smramc_pre
   | software (NextInstruction pa) => no_pre
   | hardware (ReceiveInterrupt i) => no_pre
-  | hardware (Exec o)             => (exec_pre o)
+  | hardware (Exec value)         => no_pre
   end h.
 
 Definition x86_postcondition
            {S:       Set}
            (context: x86Context S)
            (h:       Architecture S)
-           (ev:      x86Event S)
+           (ev:      x86Event)
            (h':      Architecture S)
   : Prop :=
   match ev with
   | software DisableInterrupt     => disable_interrupt_post
   | software EnableInterrupt      => enable_interrupt_post
-  | software (Write addr)         => write_post context addr
-  | software (Read addr)          => read_post addr
+  | software (Write addr value)   => write_post context addr
+  | software (Read addr value)    => read_post addr
   | software OpenSmram            => open_smram_post
   | software CloseSmram           => close_smram_post
   | software LockSmramc           => lock_smramc_post
   | software (NextInstruction pa) => nextinstr_post pa
   | hardware (ReceiveInterrupt i) => receive_interrupt_post i
-  | hardware (Exec o)             => read_post (ip (proc h))
+  | hardware (Exec value)         => read_post (ip (proc h))
   end h h'.
