src/x86/Value.v
@@ -1,0 +1,7 @@
+Require Import SpecCert.Address.
+
+Parameter Value: Type.
+Inductive Instruction: Type.
+
+Parameter decode: Value -> option Instruction.
+Parameter read_as_addr: Value -> PhysicalAddress.
